Revert "Merge branch 'develop' into 'develop'"
This reverts commit 629e8d66fbaf5a1424eb8bcf818d92cc68beff51

Channel.thy
@@ -7,7 +7,11 @@ text {*This is the total set of channels. While representing an existing network
  one should add here all channels that occur in the whole network.*}
 
 datatype channel = c1 | c2 | c3 | c4 | c5 | c6 | c7 | c8 | c9 | c10
-             (* for ABP Specification*) | as | ds | ar | dr | abpIn | abpOut | \<CC> string
+             (* for ABP Specification*) | c_as | c_ds | c_ar | c_dr | c_abpIn | c_abpOut
+(*
+datatype channel = \<C> string
+*)
+
 
 default_sort type
 
@@ -107,7 +111,7 @@ by (meson M.inject(2) f_inv_into_f rangeI)
 
 *)
   
-  (*
+
 instantiation channel :: finite
 begin
   instance
@@ -128,6 +132,6 @@ begin
       by (simp add: f1)  
   qed
 end   
-  *)
-  
+
+
 end
