ROOT
@@ -4,36 +4,47 @@ session "uClasses" (mustWork) = "HOLCF" +
     UnivClasses
 
 session "ubundle" (mustWork) = "uClasses" +
-  options [quick_and_dirty = false]
+  options [quick_and_dirty = true]
   theories
     UBundle
     UBundle_Conc
 
 session "ufun" (mustWork) = "uClasses" +
-  options [quick_and_dirty = false]
+  options [quick_and_dirty = true]
   theories
     UFun
     UFun_applyIn
     UFun_Comp
 
 session "uspec" (mustWork) = "uClasses" +
-  options [quick_and_dirty = false]
+  options [quick_and_dirty = true]
   theories
     USpec
 
 
 session "sb" (mustWork) = "ubundle" +
-  options [quick_and_dirty = false]
+  options [quick_and_dirty = true]
   theories
     "untimed/SB"
 
 session "spf" (mustWork) = "sb" + 
-  options [quick_and_dirty = false]
-  theories
-    "untimed/SPF"
-    "untimed/SpfStep"
-
-session "automaton" (mustWork) = "spf" + 
   options [quick_and_dirty = true]
   theories
-    "untimed/CaseStudy/Automaton"
+    "untimed/SPF"
+
+
+
+session "ubundle_opt" (canFail) = "uClasses" +
+  options [quick_and_dirty = false]
+  theories
+    UBundle
+
+session "ufun_opt" (canFail) = "uClasses" +
+  options [quick_and_dirty = false]
+  theories
+    UFun
+
+session "uspec_opt" (canFail) = "uClasses" +
+  options [quick_and_dirty = false]
+  theories
+    USpec
